Safekeeping checkin:  use FStar.Bytes and exercise a parser

src/lowparse/LowParseExample.fst
@@ -1,5 +1,8 @@
 module LowParseExample
 
+open FStar.HyperStack.ST
+open FStar.Bytes
+
 let f (input: FStar.Bytes.bytes) : Tot (option (LowParseExample.Aux.t * FStar.UInt32.t)) =
   LowParseExample.Aux.parse32_t input
 
@@ -15,4 +18,30 @@ let m (x: LowParseExample.Aux.t) : Tot FStar.Bytes.bytes =
 let s (x: LowParse.SLow.array LowParseExample.Aux.t 18) : Tot FStar.Bytes.bytes =
   LowParseExample.Aux.serialize32_t_array x
 
-let main () : Tot FStar.Int32.t = 0l
+#reset-options "--using_facts_from '* -LowParse'"
+let test (_:unit): Stack unit (fun _ -> true) (fun _ _ _ -> true) =
+  push_frame();
+  let test1 = "01020304" in
+  let testbytes = bytes_of_hex test1 in
+  let result = f testbytes in 
+  pop_frame()
+
+// BUGBUG: HACK for Kremlin kremlib issue
+// Dummy function, to call some FStar.Bytes functions.  This
+// causes Kremlin to emit type declarations that are needed bytes
+// krembytes.h.
+let dummy (_:unit): Stack unit (fun _ -> true) (fun _ _ _ -> true) =
+  assume false;
+  push_frame();
+  let p = twobytes (0uy, 1uy) in
+  let p = split p 1ul in
+  let p = iutf8_opt (utf8_encode "Napoléon") in
+  pop_frame()
+
+val main: Int32.t -> FStar.Buffer.buffer (FStar.Buffer.buffer C.char) ->
+  Stack C.exit_code (fun _ -> true) (fun _ _ _ -> true)
+let main argc argv =
+  push_frame ();
+  test ();
+  pop_frame ();
+  C.EXIT_SUCCESS
